add new files

_src06052011/flexClass.v
@@ -13,7 +13,7 @@ Require Import FinProof.StateMonad21.
 
 (* Require Import FinProof.Lib.BasicModuleTypes. *)
 Require Import UMLang.SolidityNotations2.
-Require Import UMLang.SML_NG24.
+Require Import UMLang.SML_NG20.
 (* Require Import flexTypes. *)
 
 Section RecordsDefinitions.
@@ -47,10 +47,7 @@ Notation " 'fst12' x " := ( fst ( fst11 x ) ) (at level 60, right associativity)
 Notation " 'fst13' x " := ( fst ( fst12 x ) ) (at level 60, right associativity).
 
 
-
-
-
-Inductive Tip3Config := 
+Inductive Tip3Config :=
 | Tip3Config_ι_name 
 | Tip3Config_ι_symbol 
 | Tip3Config_ι_decimals 
@@ -58,12 +55,13 @@ Inductive Tip3Config :=
 | Tip3Config_ι_root_address 
 | Tip3Config_ι_code 
 
-. 
+.
+ 
 Definition Tip3ConfigP := ( 
 S * S * I8 * I256 * A * C )%type . 
 
  
-Definition Tip3Config_field_type f : Type :=  
+Definition Tip3Config_get : forall (f: Tip3Config)(r: Tip3ConfigP ) , 
 match f with 
 | Tip3Config_ι_name => S 
 | Tip3Config_ι_symbol => S 
@@ -73,40 +71,20 @@ match f with
 | Tip3Config_ι_code => C 
 
 end . 
+ intros f r. 
+ destruct r as  ((((( d1 , d2 ), d3), d4), d5), d6) . 
+ destruct f. 
 
- 
-Definition Tip3Config_get (f: Tip3Config )(r: Tip3ConfigP ) :  Tip3Config_field_type f := 
- match f with 
-| Tip3Config_ι_name => fst5 r 
- | Tip3Config_ι_symbol => snd ( fst4 r ) 
- | Tip3Config_ι_decimals => snd ( fst3 r ) 
- | Tip3Config_ι_root_public_key => snd ( fst2 r ) 
- | Tip3Config_ι_root_address => snd ( fst1 r ) 
- | Tip3Config_ι_code => snd r 
- end . 
+ refine d1. 
+ refine d2. 
+ refine d3. 
+ refine d4. 
+ refine d5. 
+ refine d6. 
+Defined. 
 
  
 Coercion Tip3Config_get : Tip3Config >-> Funclass. 
-
- 
-Definition Tip3Config_set (f: Tip3Config ) 
-(v: Tip3Config_field_type f) (r: Tip3ConfigP ): Tip3ConfigP  :=
-  match f, v with 
-| Tip3Config_ι_name v' => ( v' , snd ( fst4 r ) , snd ( fst3 r ) , snd ( fst2 r ) , snd ( fst1 r ) , snd r ) 
- | Tip3Config_ι_symbol v' => ( fst5 , v' , snd ( fst3 r ) , snd ( fst2 r ) , snd ( fst1 r ) , snd r ) 
- | Tip3Config_ι_decimals v' => ( fst5 , snd ( fst4 r ) , v' , snd ( fst2 r ) , snd ( fst1 r ) , snd r ) 
- | Tip3Config_ι_root_public_key v' => ( fst5 , snd ( fst4 r ) , snd ( fst3 r ) , v' , snd ( fst1 r ) , snd r ) 
- | Tip3Config_ι_root_address v' => ( fst5 , snd ( fst4 r ) , snd ( fst3 r ) , snd ( fst2 r ) , v' , snd r ) 
- | Tip3Config_ι_code v' => ( fst5 , snd ( fst4 r ) , snd ( fst3 r ) , snd ( fst2 r ) , snd ( fst1 r ) , v' ) 
- end . 
-
- 
-Global Instance Tip3Config_set_Record : PruvendoRecord Tip3ConfigP Tip3ConfigFields :=
-{
-  field_type := Tip3Config_field_type; 
-  getPruvendoRecord := @Tip3Config_get ;
-  setPruvendoRecord := @Tip3Config_set ;
-}. 
 
  
 Inductive OrderRet := 
@@ -119,41 +97,23 @@ Definition OrderRetP := (
 I32 * I128 * I128 )%type . 
 
  
-Definition OrderRet_field_type f : Type :=  
+Definition OrderRet_get : forall (f: OrderRet)(r: OrderRetP ) , 
 match f with 
 | OrderRet_ι_err_code => I32 
 | OrderRet_ι_processed => I128 
 | OrderRet_ι_enqueued => I128 
 
 end . 
+ intros f r. 
+ destruct r as  (( d1 , d2 ), d3) . 
+ destruct f. 
 
- 
-Definition OrderRet_get (f: OrderRet )(r: OrderRetP ) :  OrderRet_field_type f := 
- match f with 
-| OrderRet_ι_err_code => fst2 r 
- | OrderRet_ι_processed => snd ( fst1 r ) 
- | OrderRet_ι_enqueued => snd r 
- end . 
+ refine d1. 
+ refine d2. 
+ refine d3. Defined. 
 
  
 Coercion OrderRet_get : OrderRet >-> Funclass. 
-
- 
-Definition OrderRet_set (f: OrderRet ) 
-(v: OrderRet_field_type f) (r: OrderRetP ): OrderRetP  :=
-  match f, v with 
-| OrderRet_ι_err_code v' => ( v' , snd ( fst1 r ) , snd r ) 
- | OrderRet_ι_processed v' => ( fst2 , v' , snd r ) 
- | OrderRet_ι_enqueued v' => ( fst2 , snd ( fst1 r ) , v' ) 
- end . 
-
- 
-Global Instance OrderRet_set_Record : PruvendoRecord OrderRetP OrderRetFields :=
-{
-  field_type := OrderRet_field_type; 
-  getPruvendoRecord := @OrderRet_get ;
-  setPruvendoRecord := @OrderRet_set ;
-}. 
 
  
 Inductive SellArgs := 
@@ -161,42 +121,26 @@ Inductive SellArgs :=
 | SellArgs_ι_receive_wallet 
 
 . 
+
 Definition SellArgsP := ( 
 I128 * addr_std_fixedP )%type . 
 
  
-Definition SellArgs_field_type f : Type :=  
+Definition SellArgs_get : forall (f: SellArgs)(r: SellArgsP ) , 
 match f with 
 | SellArgs_ι_amount => I128 
 | SellArgs_ι_receive_wallet => addr_std_fixedP 
 
 end . 
+ intros f r. 
+ destruct r as  ( d1 , d2 ) . 
+ destruct f. 
 
- 
-Definition SellArgs_get (f: SellArgs )(r: SellArgsP ) :  SellArgs_field_type f := 
- match f with 
-| SellArgs_ι_amount => fst1 r 
- | SellArgs_ι_receive_wallet => snd r 
- end . 
+ refine d1. 
+ refine d2. Defined. 
 
  
 Coercion SellArgs_get : SellArgs >-> Funclass. 
-
- 
-Definition SellArgs_set (f: SellArgs ) 
-(v: SellArgs_field_type f) (r: SellArgsP ): SellArgsP  :=
-  match f, v with 
-| SellArgs_ι_amount v' => ( v' , snd r ) 
- | SellArgs_ι_receive_wallet v' => ( fst1 , v' ) 
- end . 
-
- 
-Global Instance SellArgs_set_Record : PruvendoRecord SellArgsP SellArgsFields :=
-{
-  field_type := SellArgs_field_type; 
-  getPruvendoRecord := @SellArgs_get ;
-  setPruvendoRecord := @SellArgs_set ;
-}. 
 
  
 Inductive SellInfo := 
@@ -212,7 +156,7 @@ Definition SellInfoP := (
 I128 * I128 * I128 * addr_std_fixedP * addr_std_fixedP * I32 )%type . 
 
  
-Definition SellInfo_field_type f : Type :=  
+Definition SellInfo_get : forall (f: SellInfo)(r: SellInfoP ) , 
 match f with 
 | SellInfo_ι_original_amount => I128 
 | SellInfo_ι_amount => I128 
@@ -222,40 +166,19 @@ match f with
 | SellInfo_ι_lend_finish_time => I32 
 
 end . 
+ intros f r. 
+ destruct r as  ((((( d1 , d2 ), d3), d4), d5), d6) . 
+ destruct f. 
 
- 
-Definition SellInfo_get (f: SellInfo )(r: SellInfoP ) :  SellInfo_field_type f := 
- match f with 
-| SellInfo_ι_original_amount => fst5 r 
- | SellInfo_ι_amount => snd ( fst4 r ) 
- | SellInfo_ι_account => snd ( fst3 r ) 
- | SellInfo_ι_tip3_wallet => snd ( fst2 r ) 
- | SellInfo_ι_receive_wallet => snd ( fst1 r ) 
- | SellInfo_ι_lend_finish_time => snd r 
- end . 
+ refine d1. 
+ refine d2. 
+ refine d3. 
+ refine d4. 
+ refine d5. 
+ refine d6. Defined. 
 
  
 Coercion SellInfo_get : SellInfo >-> Funclass. 
-
- 
-Definition SellInfo_set (f: SellInfo ) 
-(v: SellInfo_field_type f) (r: SellInfoP ): SellInfoP  :=
-  match f, v with 
-| SellInfo_ι_original_amount v' => ( v' , snd ( fst4 r ) , snd ( fst3 r ) , snd ( fst2 r ) , snd ( fst1 r ) , snd r ) 
- | SellInfo_ι_amount v' => ( fst5 , v' , snd ( fst3 r ) , snd ( fst2 r ) , snd ( fst1 r ) , snd r ) 
- | SellInfo_ι_account v' => ( fst5 , snd ( fst4 r ) , v' , snd ( fst2 r ) , snd ( fst1 r ) , snd r ) 
- | SellInfo_ι_tip3_wallet v' => ( fst5 , snd ( fst4 r ) , snd ( fst3 r ) , v' , snd ( fst1 r ) , snd r ) 
- | SellInfo_ι_receive_wallet v' => ( fst5 , snd ( fst4 r ) , snd ( fst3 r ) , snd ( fst2 r ) , v' , snd r ) 
- | SellInfo_ι_lend_finish_time v' => ( fst5 , snd ( fst4 r ) , snd ( fst3 r ) , snd ( fst2 r ) , snd ( fst1 r ) , v' ) 
- end . 
-
- 
-Global Instance SellInfo_set_Record : PruvendoRecord SellInfoP SellInfoFields :=
-{
-  field_type := SellInfo_field_type; 
-  getPruvendoRecord := @SellInfo_get ;
-  setPruvendoRecord := @SellInfo_set ;
-}. 
 
  
 Inductive BuyInfo := 
@@ -270,7 +193,7 @@ Definition BuyInfoP := (
 I128 * I128 * I128 * addr_std_fixedP * addr_std_fixedP )%type . 
 
  
-Definition BuyInfo_field_type f : Type :=  
+Definition BuyInfo_get : forall (f: BuyInfo)(r: BuyInfoP ) , 
 match f with 
 | BuyInfo_ι_original_amount => I128 
 | BuyInfo_ι_amount => I128 
@@ -279,38 +202,18 @@ match f with
 | BuyInfo_ι_answer_addr => addr_std_fixedP 
 
 end . 
+ intros f r. 
+ destruct r as  (((( d1 , d2 ), d3), d4), d5) . 
+ destruct f. 
 
- 
-Definition BuyInfo_get (f: BuyInfo )(r: BuyInfoP ) :  BuyInfo_field_type f := 
- match f with 
-| BuyInfo_ι_original_amount => fst4 r 
- | BuyInfo_ι_amount => snd ( fst3 r ) 
- | BuyInfo_ι_account => snd ( fst2 r ) 
- | BuyInfo_ι_receive_tip3_wallet => snd ( fst1 r ) 
- | BuyInfo_ι_answer_addr => snd r 
- end . 
+ refine d1. 
+ refine d2. 
+ refine d3. 
+ refine d4. 
+ refine d5. Defined. 
 
  
 Coercion BuyInfo_get : BuyInfo >-> Funclass. 
-
- 
-Definition BuyInfo_set (f: BuyInfo ) 
-(v: BuyInfo_field_type f) (r: BuyInfoP ): BuyInfoP  :=
-  match f, v with 
-| BuyInfo_ι_original_amount v' => ( v' , snd ( fst3 r ) , snd ( fst2 r ) , snd ( fst1 r ) , snd r ) 
- | BuyInfo_ι_amount v' => ( fst4 , v' , snd ( fst2 r ) , snd ( fst1 r ) , snd r ) 
- | BuyInfo_ι_account v' => ( fst4 , snd ( fst3 r ) , v' , snd ( fst1 r ) , snd r ) 
- | BuyInfo_ι_receive_tip3_wallet v' => ( fst4 , snd ( fst3 r ) , snd ( fst2 r ) , v' , snd r ) 
- | BuyInfo_ι_answer_addr v' => ( fst4 , snd ( fst3 r ) , snd ( fst2 r ) , snd ( fst1 r ) , v' ) 
- end . 
-
- 
-Global Instance BuyInfo_set_Record : PruvendoRecord BuyInfoP BuyInfoFields :=
-{
-  field_type := BuyInfo_field_type; 
-  getPruvendoRecord := @BuyInfo_get ;
-  setPruvendoRecord := @BuyInfo_set ;
-}. 
 
  
 Inductive DetailsInfo := 
@@ -324,7 +227,7 @@ Definition DetailsInfoP := (
 I128 * I128 * I128 * I128 )%type . 
 
  
-Definition DetailsInfo_field_type f : Type :=  
+Definition DetailsInfo_get : forall (f: DetailsInfo)(r: DetailsInfoP ) , 
 match f with 
 | DetailsInfo_ι_price => I128 
 | DetailsInfo_ι_min_amount => I128 
@@ -332,36 +235,17 @@ match f with
 | DetailsInfo_ι_buy_amount => I128 
 
 end . 
+ intros f r. 
+ destruct r as  ((( d1 , d2 ), d3), d4) . 
+ destruct f. 
 
- 
-Definition DetailsInfo_get (f: DetailsInfo )(r: DetailsInfoP ) :  DetailsInfo_field_type f := 
- match f with 
-| DetailsInfo_ι_price => fst3 r 
- | DetailsInfo_ι_min_amount => snd ( fst2 r ) 
- | DetailsInfo_ι_sell_amount => snd ( fst1 r ) 
- | DetailsInfo_ι_buy_amount => snd r 
- end . 
+ refine d1. 
+ refine d2. 
+ refine d3. 
+ refine d4. Defined. 
 
  
 Coercion DetailsInfo_get : DetailsInfo >-> Funclass. 
-
- 
-Definition DetailsInfo_set (f: DetailsInfo ) 
-(v: DetailsInfo_field_type f) (r: DetailsInfoP ): DetailsInfoP  :=
-  match f, v with 
-| DetailsInfo_ι_price v' => ( v' , snd ( fst2 r ) , snd ( fst1 r ) , snd r ) 
- | DetailsInfo_ι_min_amount v' => ( fst3 , v' , snd ( fst1 r ) , snd r ) 
- | DetailsInfo_ι_sell_amount v' => ( fst3 , snd ( fst2 r ) , v' , snd r ) 
- | DetailsInfo_ι_buy_amount v' => ( fst3 , snd ( fst2 r ) , snd ( fst1 r ) , v' ) 
- end . 
-
- 
-Global Instance DetailsInfo_set_Record : PruvendoRecord DetailsInfoP DetailsInfoFields :=
-{
-  field_type := DetailsInfo_field_type; 
-  getPruvendoRecord := @DetailsInfo_get ;
-  setPruvendoRecord := @DetailsInfo_set ;
-}. 
 
  
 Inductive DPrice := 
@@ -375,15 +259,17 @@ Inductive DPrice :=
 | DPrice_ι_workchain_id_ 
 | DPrice_ι_tons_cfg_ 
 | DPrice_ι_tip3cfg_ 
-| DPrice_ι_sells_ 
-| DPrice_ι_buys_ 
 
 . 
+
+Definition TonsConfigP := ( 
+I128 * I128 * I128 * I128 * I128 * I128 )%type . 
+
 Definition DPriceP := ( 
-I128 * I128 * I128 * addr_std_fixedP * I128 * I8 * IStockNotifyPtrP * I8 * TonsConfigP * Tip3ConfigP * Q SellInfoP * Q BuyInfoP )%type . 
+I128 * I128 * I128 * addr_std_fixedP * I128 * I8 * IStockNotifyPtrP * I8 * TonsConfigP * Tip3ConfigP )%type . 
 
  
-Definition DPrice_field_type f : Type :=  
+Definition DPrice_get : forall (f: DPrice)(r: DPriceP ) , 
 match f with 
 | DPrice_ι_price_ => I128 
 | DPrice_ι_sells_amount_ => I128 
@@ -395,56 +281,26 @@ match f with
 | DPrice_ι_workchain_id_ => I8 
 | DPrice_ι_tons_cfg_ => TonsConfigP 
 | DPrice_ι_tip3cfg_ => Tip3ConfigP 
-| DPrice_ι_sells_ => Q SellInfoP 
-| DPrice_ι_buys_ => Q BuyInfoP 
 
 end . 
+ intros f r. 
+ destruct r as  ((((((((( d1 , d2 ), d3), d4), d5), d6), d7), d8), d9), d10) . 
+ destruct f. 
 
- 
-Definition DPrice_get (f: DPrice )(r: DPriceP ) :  DPrice_field_type f := 
- match f with 
-| DPrice_ι_price_ => fst11 r 
- | DPrice_ι_sells_amount_ => snd ( fst10 r ) 
- | DPrice_ι_buys_amount_ => snd ( fst9 r ) 
- | DPrice_ι_stock_ => snd ( fst8 r ) 
- | DPrice_ι_min_amount_ => snd ( fst7 r ) 
- | DPrice_ι_deals_limit_ => snd ( fst6 r ) 
- | DPrice_ι_notify_addr_ => snd ( fst5 r ) 
- | DPrice_ι_workchain_id_ => snd ( fst4 r ) 
- | DPrice_ι_tons_cfg_ => snd ( fst3 r ) 
- | DPrice_ι_tip3cfg_ => snd ( fst2 r ) 
- | DPrice_ι_sells_ => snd ( fst1 r ) 
- | DPrice_ι_buys_ => snd r 
- end . 
+ refine d1. 
+ refine d2. 
+ refine d3. 
+ refine d4. 
+ refine d5. 
+ refine d6. 
+ refine d7. 
+ refine d8. 
+ refine d9. 
+ refine d10. 
+Defined. 
 
  
 Coercion DPrice_get : DPrice >-> Funclass. 
-
- 
-Definition DPrice_set (f: DPrice ) 
-(v: DPrice_field_type f) (r: DPriceP ): DPriceP  :=
-  match f, v with 
-| DPrice_ι_price_ v' => ( v' , snd ( fst10 r ) , snd ( fst9 r ) , snd ( fst8 r ) , snd ( fst7 r ) , snd ( fst6 r ) , snd ( fst5 r ) , snd ( fst4 r ) , snd ( fst3 r ) , snd ( fst2 r ) , snd ( fst1 r ) , snd r ) 
- | DPrice_ι_sells_amount_ v' => ( fst11 , v' , snd ( fst9 r ) , snd ( fst8 r ) , snd ( fst7 r ) , snd ( fst6 r ) , snd ( fst5 r ) , snd ( fst4 r ) , snd ( fst3 r ) , snd ( fst2 r ) , snd ( fst1 r ) , snd r ) 
- | DPrice_ι_buys_amount_ v' => ( fst11 , snd ( fst10 r ) , v' , snd ( fst8 r ) , snd ( fst7 r ) , snd ( fst6 r ) , snd ( fst5 r ) , snd ( fst4 r ) , snd ( fst3 r ) , snd ( fst2 r ) , snd ( fst1 r ) , snd r ) 
- | DPrice_ι_stock_ v' => ( fst11 , snd ( fst10 r ) , snd ( fst9 r ) , v' , snd ( fst7 r ) , snd ( fst6 r ) , snd ( fst5 r ) , snd ( fst4 r ) , snd ( fst3 r ) , snd ( fst2 r ) , snd ( fst1 r ) , snd r ) 
- | DPrice_ι_min_amount_ v' => ( fst11 , snd ( fst10 r ) , snd ( fst9 r ) , snd ( fst8 r ) , v' , snd ( fst6 r ) , snd ( fst5 r ) , snd ( fst4 r ) , snd ( fst3 r ) , snd ( fst2 r ) , snd ( fst1 r ) , snd r ) 
- | DPrice_ι_deals_limit_ v' => ( fst11 , snd ( fst10 r ) , snd ( fst9 r ) , snd ( fst8 r ) , snd ( fst7 r ) , v' , snd ( fst5 r ) , snd ( fst4 r ) , snd ( fst3 r ) , snd ( fst2 r ) , snd ( fst1 r ) , snd r ) 
- | DPrice_ι_notify_addr_ v' => ( fst11 , snd ( fst10 r ) , snd ( fst9 r ) , snd ( fst8 r ) , snd ( fst7 r ) , snd ( fst6 r ) , v' , snd ( fst4 r ) , snd ( fst3 r ) , snd ( fst2 r ) , snd ( fst1 r ) , snd r ) 
- | DPrice_ι_workchain_id_ v' => ( fst11 , snd ( fst10 r ) , snd ( fst9 r ) , snd ( fst8 r ) , snd ( fst7 r ) , snd ( fst6 r ) , snd ( fst5 r ) , v' , snd ( fst3 r ) , snd ( fst2 r ) , snd ( fst1 r ) , snd r ) 
- | DPrice_ι_tons_cfg_ v' => ( fst11 , snd ( fst10 r ) , snd ( fst9 r ) , snd ( fst8 r ) , snd ( fst7 r ) , snd ( fst6 r ) , snd ( fst5 r ) , snd ( fst4 r ) , v' , snd ( fst2 r ) , snd ( fst1 r ) , snd r ) 
- | DPrice_ι_tip3cfg_ v' => ( fst11 , snd ( fst10 r ) , snd ( fst9 r ) , snd ( fst8 r ) , snd ( fst7 r ) , snd ( fst6 r ) , snd ( fst5 r ) , snd ( fst4 r ) , snd ( fst3 r ) , v' , snd ( fst1 r ) , snd r ) 
- | DPrice_ι_sells_ v' => ( fst11 , snd ( fst10 r ) , snd ( fst9 r ) , snd ( fst8 r ) , snd ( fst7 r ) , snd ( fst6 r ) , snd ( fst5 r ) , snd ( fst4 r ) , snd ( fst3 r ) , snd ( fst2 r ) , v' , snd r ) 
- | DPrice_ι_buys_ v' => ( fst11 , snd ( fst10 r ) , snd ( fst9 r ) , snd ( fst8 r ) , snd ( fst7 r ) , snd ( fst6 r ) , snd ( fst5 r ) , snd ( fst4 r ) , snd ( fst3 r ) , snd ( fst2 r ) , snd ( fst1 r ) , v' ) 
- end . 
-
- 
-Global Instance DPrice_set_Record : PruvendoRecord DPriceP DPriceFields :=
-{
-  field_type := DPrice_field_type; 
-  getPruvendoRecord := @DPrice_get ;
-  setPruvendoRecord := @DPrice_set ;
-}. 
 
  
 Inductive TonsConfig := 
@@ -454,13 +310,11 @@ Inductive TonsConfig :=
 | TonsConfig_ι_order_answer 
 | TonsConfig_ι_process_queue 
 | TonsConfig_ι_send_notify 
+.
 
-. 
-Definition TonsConfigP := ( 
-I128 * I128 * I128 * I128 * I128 * I128 )%type . 
 
  
-Definition TonsConfig_field_type f : Type :=  
+Definition TonsConfig_get : forall (f: TonsConfig)(r: TonsConfigP ) , 
 match f with 
 | TonsConfig_ι_transfer_tip3 => I128 
 | TonsConfig_ι_return_ownership => I128 
@@ -470,103 +324,56 @@ match f with
 | TonsConfig_ι_send_notify => I128 
 
 end . 
+ intros f r. 
+ destruct r as  ((((( d1 , d2 ), d3), d4), d5), d6) . 
+ destruct f. 
 
- 
-Definition TonsConfig_get (f: TonsConfig )(r: TonsConfigP ) :  TonsConfig_field_type f := 
- match f with 
-| TonsConfig_ι_transfer_tip3 => fst5 r 
- | TonsConfig_ι_return_ownership => snd ( fst4 r ) 
- | TonsConfig_ι_trading_pair_deploy => snd ( fst3 r ) 
- | TonsConfig_ι_order_answer => snd ( fst2 r ) 
- | TonsConfig_ι_process_queue => snd ( fst1 r ) 
- | TonsConfig_ι_send_notify => snd r 
- end . 
+ refine d1. 
+ refine d2. 
+ refine d3. 
+ refine d4. 
+ refine d5. 
+ refine d6. 
+Defined. 
 
  
 Coercion TonsConfig_get : TonsConfig >-> Funclass. 
 
  
-Definition TonsConfig_set (f: TonsConfig ) 
-(v: TonsConfig_field_type f) (r: TonsConfigP ): TonsConfigP  :=
-  match f, v with 
-| TonsConfig_ι_transfer_tip3 v' => ( v' , snd ( fst4 r ) , snd ( fst3 r ) , snd ( fst2 r ) , snd ( fst1 r ) , snd r ) 
- | TonsConfig_ι_return_ownership v' => ( fst5 , v' , snd ( fst3 r ) , snd ( fst2 r ) , snd ( fst1 r ) , snd r ) 
- | TonsConfig_ι_trading_pair_deploy v' => ( fst5 , snd ( fst4 r ) , v' , snd ( fst2 r ) , snd ( fst1 r ) , snd r ) 
- | TonsConfig_ι_order_answer v' => ( fst5 , snd ( fst4 r ) , snd ( fst3 r ) , v' , snd ( fst1 r ) , snd r ) 
- | TonsConfig_ι_process_queue v' => ( fst5 , snd ( fst4 r ) , snd ( fst3 r ) , snd ( fst2 r ) , v' , snd r ) 
- | TonsConfig_ι_send_notify v' => ( fst5 , snd ( fst4 r ) , snd ( fst3 r ) , snd ( fst2 r ) , snd ( fst1 r ) , v' ) 
- end . 
-
- 
-Global Instance TonsConfig_set_Record : PruvendoRecord TonsConfigP TonsConfigFields :=
-{
-  field_type := TonsConfig_field_type; 
-  getPruvendoRecord := @TonsConfig_get ;
-  setPruvendoRecord := @TonsConfig_set ;
-}. 
-
- 
 Inductive DStock := 
 | DStock_ι_deployer_pubkey_ 
 | DStock_ι_tons_cfg_ 
-| DStock_ι_pair_code_ 
-| DStock_ι_price_code_ 
 | DStock_ι_min_amount_ 
 | DStock_ι_deals_limit_ 
 | DStock_ι_notify_addr_ 
 
 . 
 Definition DStockP := ( 
-I256 * TonsConfigP * M C * M C * I128 * I8 * A )%type . 
+I256 * TonsConfigP * I128 * I8 * A )%type . 
 
  
-Definition DStock_field_type f : Type :=  
+Definition DStock_get : forall (f: DStock)(r: DStockP ) , 
 match f with 
 | DStock_ι_deployer_pubkey_ => I256 
 | DStock_ι_tons_cfg_ => TonsConfigP 
-| DStock_ι_pair_code_ => M C 
-| DStock_ι_price_code_ => M C 
 | DStock_ι_min_amount_ => I128 
 | DStock_ι_deals_limit_ => I8 
 | DStock_ι_notify_addr_ => A 
 
 end . 
+ intros f r. 
+ destruct r as  (((( d1 , d2 ), d3), d4), d5) . 
+ destruct f. 
 
- 
-Definition DStock_get (f: DStock )(r: DStockP ) :  DStock_field_type f := 
- match f with 
-| DStock_ι_deployer_pubkey_ => fst6 r 
- | DStock_ι_tons_cfg_ => snd ( fst5 r ) 
- | DStock_ι_pair_code_ => snd ( fst4 r ) 
- | DStock_ι_price_code_ => snd ( fst3 r ) 
- | DStock_ι_min_amount_ => snd ( fst2 r ) 
- | DStock_ι_deals_limit_ => snd ( fst1 r ) 
- | DStock_ι_notify_addr_ => snd r 
- end . 
+ refine d1. 
+ refine d2. 
+ refine d3. 
+ refine d4. 
+ refine d5. 
+Defined. 
 
  
 Coercion DStock_get : DStock >-> Funclass. 
-
- 
-Definition DStock_set (f: DStock ) 
-(v: DStock_field_type f) (r: DStockP ): DStockP  :=
-  match f, v with 
-| DStock_ι_deployer_pubkey_ v' => ( v' , snd ( fst5 r ) , snd ( fst4 r ) , snd ( fst3 r ) , snd ( fst2 r ) , snd ( fst1 r ) , snd r ) 
- | DStock_ι_tons_cfg_ v' => ( fst6 , v' , snd ( fst4 r ) , snd ( fst3 r ) , snd ( fst2 r ) , snd ( fst1 r ) , snd r ) 
- | DStock_ι_pair_code_ v' => ( fst6 , snd ( fst5 r ) , v' , snd ( fst3 r ) , snd ( fst2 r ) , snd ( fst1 r ) , snd r ) 
- | DStock_ι_price_code_ v' => ( fst6 , snd ( fst5 r ) , snd ( fst4 r ) , v' , snd ( fst2 r ) , snd ( fst1 r ) , snd r ) 
- | DStock_ι_min_amount_ v' => ( fst6 , snd ( fst5 r ) , snd ( fst4 r ) , snd ( fst3 r ) , v' , snd ( fst1 r ) , snd r ) 
- | DStock_ι_deals_limit_ v' => ( fst6 , snd ( fst5 r ) , snd ( fst4 r ) , snd ( fst3 r ) , snd ( fst2 r ) , v' , snd r ) 
- | DStock_ι_notify_addr_ v' => ( fst6 , snd ( fst5 r ) , snd ( fst4 r ) , snd ( fst3 r ) , snd ( fst2 r ) , snd ( fst1 r ) , v' ) 
- end . 
-
- 
-Global Instance DStock_set_Record : PruvendoRecord DStockP DStockFields :=
-{
-  field_type := DStock_field_type; 
-  getPruvendoRecord := @DStock_get ;
-  setPruvendoRecord := @DStock_set ;
-}. 
 
  
 Inductive DTradingPair := 
@@ -579,41 +386,24 @@ Definition DTradingPairP := (
 A * A * I128 )%type . 
 
  
-Definition DTradingPair_field_type f : Type :=  
+Definition DTradingPair_get : forall (f: DTradingPair)(r: DTradingPairP ) , 
 match f with 
 | DTradingPair_ι_stock_addr_ => A 
 | DTradingPair_ι_tip3_root_ => A 
 | DTradingPair_ι_deploy_value_ => I128 
 
 end . 
+ intros f r. 
+ destruct r as  (( d1 , d2 ), d3) . 
+ destruct f. 
 
- 
-Definition DTradingPair_get (f: DTradingPair )(r: DTradingPairP ) :  DTradingPair_field_type f := 
- match f with 
-| DTradingPair_ι_stock_addr_ => fst2 r 
- | DTradingPair_ι_tip3_root_ => snd ( fst1 r ) 
- | DTradingPair_ι_deploy_value_ => snd r 
- end . 
+ refine d1. 
+ refine d2. 
+ refine d3. 
+Defined. 
 
  
 Coercion DTradingPair_get : DTradingPair >-> Funclass. 
-
- 
-Definition DTradingPair_set (f: DTradingPair ) 
-(v: DTradingPair_field_type f) (r: DTradingPairP ): DTradingPairP  :=
-  match f, v with 
-| DTradingPair_ι_stock_addr_ v' => ( v' , snd ( fst1 r ) , snd r ) 
- | DTradingPair_ι_tip3_root_ v' => ( fst2 , v' , snd r ) 
- | DTradingPair_ι_deploy_value_ v' => ( fst2 , snd ( fst1 r ) , v' ) 
- end . 
-
- 
-Global Instance DTradingPair_set_Record : PruvendoRecord DTradingPairP DTradingPairFields :=
-{
-  field_type := DTradingPair_field_type; 
-  getPruvendoRecord := @DTradingPair_get ;
-  setPruvendoRecord := @DTradingPair_set ;
-}. 
 
  
 Inductive FLeXSellArgsAddrs := 
@@ -625,38 +415,22 @@ Definition FLeXSellArgsAddrsP := (
 A * A )%type . 
 
  
-Definition FLeXSellArgsAddrs_field_type f : Type :=  
+Definition FLeXSellArgsAddrs_get : forall (f: FLeXSellArgsAddrs)(r: FLeXSellArgsAddrsP ) , 
 match f with 
 | FLeXSellArgsAddrs_ι_my_tip3_addr => A 
 | FLeXSellArgsAddrs_ι_receive_wallet => A 
 
 end . 
+ intros f r. 
+ destruct r as  ( d1 , d2 ) . 
+ destruct f. 
 
- 
-Definition FLeXSellArgsAddrs_get (f: FLeXSellArgsAddrs )(r: FLeXSellArgsAddrsP ) :  FLeXSellArgsAddrs_field_type f := 
- match f with 
-| FLeXSellArgsAddrs_ι_my_tip3_addr => fst1 r 
- | FLeXSellArgsAddrs_ι_receive_wallet => snd r 
- end . 
+ refine d1. 
+ refine d2. 
+Defined. 
 
  
 Coercion FLeXSellArgsAddrs_get : FLeXSellArgsAddrs >-> Funclass. 
-
- 
-Definition FLeXSellArgsAddrs_set (f: FLeXSellArgsAddrs ) 
-(v: FLeXSellArgsAddrs_field_type f) (r: FLeXSellArgsAddrsP ): FLeXSellArgsAddrsP  :=
-  match f, v with 
-| FLeXSellArgsAddrs_ι_my_tip3_addr v' => ( v' , snd r ) 
- | FLeXSellArgsAddrs_ι_receive_wallet v' => ( fst1 , v' ) 
- end . 
-
- 
-Global Instance FLeXSellArgsAddrs_set_Record : PruvendoRecord FLeXSellArgsAddrsP FLeXSellArgsAddrsFields :=
-{
-  field_type := FLeXSellArgsAddrs_field_type; 
-  getPruvendoRecord := @FLeXSellArgsAddrs_get ;
-  setPruvendoRecord := @FLeXSellArgsAddrs_set ;
-}. 
 
  
 Inductive FLeXSellArgs := 
@@ -667,15 +441,13 @@ Inductive FLeXSellArgs :=
 | FLeXSellArgs_ι_deals_limit 
 | FLeXSellArgs_ι_tons_value 
 | FLeXSellArgs_ι_price_code 
-| FLeXSellArgs_ι_addrs 
-| FLeXSellArgs_ι_tip3cfg 
 
 . 
 Definition FLeXSellArgsP := ( 
-I128 * I128 * I32 * I128 * I8 * I128 * C * ref FLeXSellArgsAddrsP * ref Tip3ConfigP )%type . 
+I128 * I128 * I32 * I128 * I8 * I128 * C )%type . 
 
  
-Definition FLeXSellArgs_field_type f : Type :=  
+Definition FLeXSellArgs_get : forall (f: FLeXSellArgs)(r: FLeXSellArgsP ) , 
 match f with 
 | FLeXSellArgs_ι_price => I128 
 | FLeXSellArgs_ι_amount => I128 
@@ -684,50 +456,23 @@ match f with
 | FLeXSellArgs_ι_deals_limit => I8 
 | FLeXSellArgs_ι_tons_value => I128 
 | FLeXSellArgs_ι_price_code => C 
-| FLeXSellArgs_ι_addrs => ref FLeXSellArgsAddrsP 
-| FLeXSellArgs_ι_tip3cfg => ref Tip3ConfigP 
 
 end . 
+ intros f r. 
+ destruct r as  (((((( d1 , d2 ), d3), d4), d5), d6), d7) . 
+ destruct f. 
 
- 
-Definition FLeXSellArgs_get (f: FLeXSellArgs )(r: FLeXSellArgsP ) :  FLeXSellArgs_field_type f := 
- match f with 
-| FLeXSellArgs_ι_price => fst8 r 
- | FLeXSellArgs_ι_amount => snd ( fst7 r ) 
- | FLeXSellArgs_ι_lend_finish_time => snd ( fst6 r ) 
- | FLeXSellArgs_ι_min_amount => snd ( fst5 r ) 
- | FLeXSellArgs_ι_deals_limit => snd ( fst4 r ) 
- | FLeXSellArgs_ι_tons_value => snd ( fst3 r ) 
- | FLeXSellArgs_ι_price_code => snd ( fst2 r ) 
- | FLeXSellArgs_ι_addrs => snd ( fst1 r ) 
- | FLeXSellArgs_ι_tip3cfg => snd r 
- end . 
+ refine d1. 
+ refine d2. 
+ refine d3. 
+ refine d4. 
+ refine d5. 
+ refine d6. 
+ refine d7. 
+Defined. 
 
  
 Coercion FLeXSellArgs_get : FLeXSellArgs >-> Funclass. 
-
- 
-Definition FLeXSellArgs_set (f: FLeXSellArgs ) 
-(v: FLeXSellArgs_field_type f) (r: FLeXSellArgsP ): FLeXSellArgsP  :=
-  match f, v with 
-| FLeXSellArgs_ι_price v' => ( v' , snd ( fst7 r ) , snd ( fst6 r ) , snd ( fst5 r ) , snd ( fst4 r ) , snd ( fst3 r ) , snd ( fst2 r ) , snd ( fst1 r ) , snd r ) 
- | FLeXSellArgs_ι_amount v' => ( fst8 , v' , snd ( fst6 r ) , snd ( fst5 r ) , snd ( fst4 r ) , snd ( fst3 r ) , snd ( fst2 r ) , snd ( fst1 r ) , snd r ) 
- | FLeXSellArgs_ι_lend_finish_time v' => ( fst8 , snd ( fst7 r ) , v' , snd ( fst5 r ) , snd ( fst4 r ) , snd ( fst3 r ) , snd ( fst2 r ) , snd ( fst1 r ) , snd r ) 
- | FLeXSellArgs_ι_min_amount v' => ( fst8 , snd ( fst7 r ) , snd ( fst6 r ) , v' , snd ( fst4 r ) , snd ( fst3 r ) , snd ( fst2 r ) , snd ( fst1 r ) , snd r ) 
- | FLeXSellArgs_ι_deals_limit v' => ( fst8 , snd ( fst7 r ) , snd ( fst6 r ) , snd ( fst5 r ) , v' , snd ( fst3 r ) , snd ( fst2 r ) , snd ( fst1 r ) , snd r ) 
- | FLeXSellArgs_ι_tons_value v' => ( fst8 , snd ( fst7 r ) , snd ( fst6 r ) , snd ( fst5 r ) , snd ( fst4 r ) , v' , snd ( fst2 r ) , snd ( fst1 r ) , snd r ) 
- | FLeXSellArgs_ι_price_code v' => ( fst8 , snd ( fst7 r ) , snd ( fst6 r ) , snd ( fst5 r ) , snd ( fst4 r ) , snd ( fst3 r ) , v' , snd ( fst1 r ) , snd r ) 
- | FLeXSellArgs_ι_addrs v' => ( fst8 , snd ( fst7 r ) , snd ( fst6 r ) , snd ( fst5 r ) , snd ( fst4 r ) , snd ( fst3 r ) , snd ( fst2 r ) , v' , snd r ) 
- | FLeXSellArgs_ι_tip3cfg v' => ( fst8 , snd ( fst7 r ) , snd ( fst6 r ) , snd ( fst5 r ) , snd ( fst4 r ) , snd ( fst3 r ) , snd ( fst2 r ) , snd ( fst1 r ) , v' ) 
- end . 
-
- 
-Global Instance FLeXSellArgs_set_Record : PruvendoRecord FLeXSellArgsP FLeXSellArgsFields :=
-{
-  field_type := FLeXSellArgs_field_type; 
-  getPruvendoRecord := @FLeXSellArgs_get ;
-  setPruvendoRecord := @FLeXSellArgs_set ;
-}. 
 
  
 Inductive FLeXBuyArgs := 
@@ -738,14 +483,13 @@ Inductive FLeXBuyArgs :=
 | FLeXBuyArgs_ι_deploy_value 
 | FLeXBuyArgs_ι_price_code 
 | FLeXBuyArgs_ι_my_tip3_addr 
-| FLeXBuyArgs_ι_tip3cfg 
 
 . 
 Definition FLeXBuyArgsP := ( 
-I128 * I128 * I128 * I8 * I128 * C * A * ref Tip3ConfigP )%type . 
+I128 * I128 * I128 * I8 * I128 * C * A )%type . 
 
  
-Definition FLeXBuyArgs_field_type f : Type :=  
+Definition FLeXBuyArgs_get : forall (f: FLeXBuyArgs)(r: FLeXBuyArgsP ) , 
 match f with 
 | FLeXBuyArgs_ι_price => I128 
 | FLeXBuyArgs_ι_amount => I128 
@@ -754,47 +498,22 @@ match f with
 | FLeXBuyArgs_ι_deploy_value => I128 
 | FLeXBuyArgs_ι_price_code => C 
 | FLeXBuyArgs_ι_my_tip3_addr => A 
-| FLeXBuyArgs_ι_tip3cfg => ref Tip3ConfigP 
 
 end . 
+ intros f r. 
+ destruct r as  (((((( d1 , d2 ), d3), d4), d5), d6), d7) . 
+ destruct f. 
 
- 
-Definition FLeXBuyArgs_get (f: FLeXBuyArgs )(r: FLeXBuyArgsP ) :  FLeXBuyArgs_field_type f := 
- match f with 
-| FLeXBuyArgs_ι_price => fst7 r 
- | FLeXBuyArgs_ι_amount => snd ( fst6 r ) 
- | FLeXBuyArgs_ι_min_amount => snd ( fst5 r ) 
- | FLeXBuyArgs_ι_deals_limit => snd ( fst4 r ) 
- | FLeXBuyArgs_ι_deploy_value => snd ( fst3 r ) 
- | FLeXBuyArgs_ι_price_code => snd ( fst2 r ) 
- | FLeXBuyArgs_ι_my_tip3_addr => snd ( fst1 r ) 
- | FLeXBuyArgs_ι_tip3cfg => snd r 
- end . 
+ refine d1. 
+ refine d2. 
+ refine d3. 
+ refine d4. 
+ refine d5. 
+ refine d6. 
+ refine d7. Defined. 
 
  
 Coercion FLeXBuyArgs_get : FLeXBuyArgs >-> Funclass. 
-
- 
-Definition FLeXBuyArgs_set (f: FLeXBuyArgs ) 
-(v: FLeXBuyArgs_field_type f) (r: FLeXBuyArgsP ): FLeXBuyArgsP  :=
-  match f, v with 
-| FLeXBuyArgs_ι_price v' => ( v' , snd ( fst6 r ) , snd ( fst5 r ) , snd ( fst4 r ) , snd ( fst3 r ) , snd ( fst2 r ) , snd ( fst1 r ) , snd r ) 
- | FLeXBuyArgs_ι_amount v' => ( fst7 , v' , snd ( fst5 r ) , snd ( fst4 r ) , snd ( fst3 r ) , snd ( fst2 r ) , snd ( fst1 r ) , snd r ) 
- | FLeXBuyArgs_ι_min_amount v' => ( fst7 , snd ( fst6 r ) , v' , snd ( fst4 r ) , snd ( fst3 r ) , snd ( fst2 r ) , snd ( fst1 r ) , snd r ) 
- | FLeXBuyArgs_ι_deals_limit v' => ( fst7 , snd ( fst6 r ) , snd ( fst5 r ) , v' , snd ( fst3 r ) , snd ( fst2 r ) , snd ( fst1 r ) , snd r ) 
- | FLeXBuyArgs_ι_deploy_value v' => ( fst7 , snd ( fst6 r ) , snd ( fst5 r ) , snd ( fst4 r ) , v' , snd ( fst2 r ) , snd ( fst1 r ) , snd r ) 
- | FLeXBuyArgs_ι_price_code v' => ( fst7 , snd ( fst6 r ) , snd ( fst5 r ) , snd ( fst4 r ) , snd ( fst3 r ) , v' , snd ( fst1 r ) , snd r ) 
- | FLeXBuyArgs_ι_my_tip3_addr v' => ( fst7 , snd ( fst6 r ) , snd ( fst5 r ) , snd ( fst4 r ) , snd ( fst3 r ) , snd ( fst2 r ) , v' , snd r ) 
- | FLeXBuyArgs_ι_tip3cfg v' => ( fst7 , snd ( fst6 r ) , snd ( fst5 r ) , snd ( fst4 r ) , snd ( fst3 r ) , snd ( fst2 r ) , snd ( fst1 r ) , v' ) 
- end . 
-
- 
-Global Instance FLeXBuyArgs_set_Record : PruvendoRecord FLeXBuyArgsP FLeXBuyArgsFields :=
-{
-  field_type := FLeXBuyArgs_field_type; 
-  getPruvendoRecord := @FLeXBuyArgs_get ;
-  setPruvendoRecord := @FLeXBuyArgs_set ;
-}. 
 
  
 Inductive FLeXCancelArgs := 
@@ -803,57 +522,33 @@ Inductive FLeXCancelArgs :=
 | FLeXCancelArgs_ι_deals_limit 
 | FLeXCancelArgs_ι_value 
 | FLeXCancelArgs_ι_price_code 
-| FLeXCancelArgs_ι_tip3cfg 
 
 . 
 Definition FLeXCancelArgsP := ( 
-I128 * I128 * I8 * I128 * C * ref Tip3ConfigP )%type . 
+I128 * I128 * I8 * I128 * C )%type . 
 
  
-Definition FLeXCancelArgs_field_type f : Type :=  
+Definition FLeXCancelArgs_get : forall (f: FLeXCancelArgs)(r: FLeXCancelArgsP ) , 
 match f with 
 | FLeXCancelArgs_ι_price => I128 
 | FLeXCancelArgs_ι_min_amount => I128 
 | FLeXCancelArgs_ι_deals_limit => I8 
 | FLeXCancelArgs_ι_value => I128 
 | FLeXCancelArgs_ι_price_code => C 
-| FLeXCancelArgs_ι_tip3cfg => ref Tip3ConfigP 
 
 end . 
+ intros f r. 
+ destruct r as  (((( d1 , d2 ), d3), d4), d5) . 
+ destruct f. 
 
- 
-Definition FLeXCancelArgs_get (f: FLeXCancelArgs )(r: FLeXCancelArgsP ) :  FLeXCancelArgs_field_type f := 
- match f with 
-| FLeXCancelArgs_ι_price => fst5 r 
- | FLeXCancelArgs_ι_min_amount => snd ( fst4 r ) 
- | FLeXCancelArgs_ι_deals_limit => snd ( fst3 r ) 
- | FLeXCancelArgs_ι_value => snd ( fst2 r ) 
- | FLeXCancelArgs_ι_price_code => snd ( fst1 r ) 
- | FLeXCancelArgs_ι_tip3cfg => snd r 
- end . 
+ refine d1. 
+ refine d2. 
+ refine d3. 
+ refine d4. 
+ refine d5. Defined. 
 
  
 Coercion FLeXCancelArgs_get : FLeXCancelArgs >-> Funclass. 
-
- 
-Definition FLeXCancelArgs_set (f: FLeXCancelArgs ) 
-(v: FLeXCancelArgs_field_type f) (r: FLeXCancelArgsP ): FLeXCancelArgsP  :=
-  match f, v with 
-| FLeXCancelArgs_ι_price v' => ( v' , snd ( fst4 r ) , snd ( fst3 r ) , snd ( fst2 r ) , snd ( fst1 r ) , snd r ) 
- | FLeXCancelArgs_ι_min_amount v' => ( fst5 , v' , snd ( fst3 r ) , snd ( fst2 r ) , snd ( fst1 r ) , snd r ) 
- | FLeXCancelArgs_ι_deals_limit v' => ( fst5 , snd ( fst4 r ) , v' , snd ( fst2 r ) , snd ( fst1 r ) , snd r ) 
- | FLeXCancelArgs_ι_value v' => ( fst5 , snd ( fst4 r ) , snd ( fst3 r ) , v' , snd ( fst1 r ) , snd r ) 
- | FLeXCancelArgs_ι_price_code v' => ( fst5 , snd ( fst4 r ) , snd ( fst3 r ) , snd ( fst2 r ) , v' , snd r ) 
- | FLeXCancelArgs_ι_tip3cfg v' => ( fst5 , snd ( fst4 r ) , snd ( fst3 r ) , snd ( fst2 r ) , snd ( fst1 r ) , v' ) 
- end . 
-
- 
-Global Instance FLeXCancelArgs_set_Record : PruvendoRecord FLeXCancelArgsP FLeXCancelArgsFields :=
-{
-  field_type := FLeXCancelArgs_field_type; 
-  getPruvendoRecord := @FLeXCancelArgs_get ;
-  setPruvendoRecord := @FLeXCancelArgs_set ;
-}. 
 
  
 Inductive DFLeXClient := 
@@ -869,7 +564,7 @@ Definition DFLeXClientP := (
 I256 * C * I8 * TonsConfigP * A * A )%type . 
 
  
-Definition DFLeXClient_field_type f : Type :=  
+Definition DFLeXClient_get : forall (f: DFLeXClient)(r: DFLeXClientP ) , 
 match f with 
 | DFLeXClient_ι_owner_ => I256 
 | DFLeXClient_ι_trading_pair_code_ => C 
@@ -879,95 +574,45 @@ match f with
 | DFLeXClient_ι_notify_addr_ => A 
 
 end . 
+ intros f r. 
+ destruct r as  ((((( d1 , d2 ), d3), d4), d5), d6) . 
+ destruct f. 
 
- 
-Definition DFLeXClient_get (f: DFLeXClient )(r: DFLeXClientP ) :  DFLeXClient_field_type f := 
- match f with 
-| DFLeXClient_ι_owner_ => fst5 r 
- | DFLeXClient_ι_trading_pair_code_ => snd ( fst4 r ) 
- | DFLeXClient_ι_workchain_id_ => snd ( fst3 r ) 
- | DFLeXClient_ι_tons_cfg_ => snd ( fst2 r ) 
- | DFLeXClient_ι_stock_ => snd ( fst1 r ) 
- | DFLeXClient_ι_notify_addr_ => snd r 
- end . 
+ refine d1. 
+ refine d2. 
+ refine d3. 
+ refine d4. 
+ refine d5. 
+ refine d6. Defined. 
 
  
 Coercion DFLeXClient_get : DFLeXClient >-> Funclass. 
 
  
-Definition DFLeXClient_set (f: DFLeXClient ) 
-(v: DFLeXClient_field_type f) (r: DFLeXClientP ): DFLeXClientP  :=
-  match f, v with 
-| DFLeXClient_ι_owner_ v' => ( v' , snd ( fst4 r ) , snd ( fst3 r ) , snd ( fst2 r ) , snd ( fst1 r ) , snd r ) 
- | DFLeXClient_ι_trading_pair_code_ v' => ( fst5 , v' , snd ( fst3 r ) , snd ( fst2 r ) , snd ( fst1 r ) , snd r ) 
- | DFLeXClient_ι_workchain_id_ v' => ( fst5 , snd ( fst4 r ) , v' , snd ( fst2 r ) , snd ( fst1 r ) , snd r ) 
- | DFLeXClient_ι_tons_cfg_ v' => ( fst5 , snd ( fst4 r ) , snd ( fst3 r ) , v' , snd ( fst1 r ) , snd r ) 
- | DFLeXClient_ι_stock_ v' => ( fst5 , snd ( fst4 r ) , snd ( fst3 r ) , snd ( fst2 r ) , v' , snd r ) 
- | DFLeXClient_ι_notify_addr_ v' => ( fst5 , snd ( fst4 r ) , snd ( fst3 r ) , snd ( fst2 r ) , snd ( fst1 r ) , v' ) 
- end . 
-
- 
-Global Instance DFLeXClient_set_Record : PruvendoRecord DFLeXClientP DFLeXClientFields :=
-{
-  field_type := DFLeXClient_field_type; 
-  getPruvendoRecord := @DFLeXClient_get ;
-  setPruvendoRecord := @DFLeXClient_set ;
-}. 
-
- 
 Inductive process_ret := 
 | process_ret_ι_sells_amount 
-| process_ret_ι_sells_ 
 | process_ret_ι_buys_amount 
-| process_ret_ι_buys_ 
-| process_ret_ι_ret_ 
 
 . 
 Definition process_retP := ( 
-I128 * Q SellInfoP * I128 * Q BuyInfoP * M OrderRetP )%type . 
+I128 * I128 )%type . 
 
  
-Definition process_ret_field_type f : Type :=  
+Definition process_ret_get : forall (f: process_ret)(r: process_retP ) , 
 match f with 
 | process_ret_ι_sells_amount => I128 
-| process_ret_ι_sells_ => Q SellInfoP 
 | process_ret_ι_buys_amount => I128 
-| process_ret_ι_buys_ => Q BuyInfoP 
-| process_ret_ι_ret_ => M OrderRetP 
 
 end . 
+ intros f r. 
+ destruct r as  ( d1 , d2 ) . 
+ destruct f. 
 
- 
-Definition process_ret_get (f: process_ret )(r: process_retP ) :  process_ret_field_type f := 
- match f with 
-| process_ret_ι_sells_amount => fst4 r 
- | process_ret_ι_sells_ => snd ( fst3 r ) 
- | process_ret_ι_buys_amount => snd ( fst2 r ) 
- | process_ret_ι_buys_ => snd ( fst1 r ) 
- | process_ret_ι_ret_ => snd r 
- end . 
+ refine d1. 
+ refine d2. Defined. 
 
  
 Coercion process_ret_get : process_ret >-> Funclass. 
-
- 
-Definition process_ret_set (f: process_ret ) 
-(v: process_ret_field_type f) (r: process_retP ): process_retP  :=
-  match f, v with 
-| process_ret_ι_sells_amount v' => ( v' , snd ( fst3 r ) , snd ( fst2 r ) , snd ( fst1 r ) , snd r ) 
- | process_ret_ι_sells_ v' => ( fst4 , v' , snd ( fst2 r ) , snd ( fst1 r ) , snd r ) 
- | process_ret_ι_buys_amount v' => ( fst4 , snd ( fst3 r ) , v' , snd ( fst1 r ) , snd r ) 
- | process_ret_ι_buys_ v' => ( fst4 , snd ( fst3 r ) , snd ( fst2 r ) , v' , snd r ) 
- | process_ret_ι_ret_ v' => ( fst4 , snd ( fst3 r ) , snd ( fst2 r ) , snd ( fst1 r ) , v' ) 
- end . 
-
- 
-Global Instance process_ret_set_Record : PruvendoRecord process_retP process_retFields :=
-{
-  field_type := process_ret_field_type; 
-  getPruvendoRecord := @process_ret_get ;
-  setPruvendoRecord := @process_ret_set ;
-}. 
 
  
 Inductive dealer := 
@@ -984,7 +629,7 @@ Definition dealerP := (
 A * IStockNotifyPtrP * I128 * I * TonsConfigP * I128 * I128 )%type . 
 
  
-Definition dealer_field_type f : Type :=  
+Definition dealer_get : forall (f: dealer)(r: dealerP ) , 
 match f with 
 | dealer_ι_tip3root_ => A 
 | dealer_ι_notify_addr_ => IStockNotifyPtrP 
@@ -995,42 +640,22 @@ match f with
 | dealer_ι_buys_amount_ => I128 
 
 end . 
+ intros f r. 
+ destruct r as  (((((( d1 , d2 ), d3), d4), d5), d6), d7) . 
+ destruct f. 
 
- 
-Definition dealer_get (f: dealer )(r: dealerP ) :  dealer_field_type f := 
- match f with 
-| dealer_ι_tip3root_ => fst6 r 
- | dealer_ι_notify_addr_ => snd ( fst5 r ) 
- | dealer_ι_price_ => snd ( fst4 r ) 
- | dealer_ι_deals_limit_ => snd ( fst3 r ) 
- | dealer_ι_tons_cfg_ => snd ( fst2 r ) 
- | dealer_ι_sells_amount_ => snd ( fst1 r ) 
- | dealer_ι_buys_amount_ => snd r 
- end . 
+ refine d1. 
+ refine d2. 
+ refine d3. 
+ refine d4. 
+ refine d5. 
+ refine d6. 
+ refine d7. Defined. 
 
  
 Coercion dealer_get : dealer >-> Funclass. 
 
  
-Definition dealer_set (f: dealer ) 
-(v: dealer_field_type f) (r: dealerP ): dealerP  :=
-  match f, v with 
-| dealer_ι_tip3root_ v' => ( v' , snd ( fst5 r ) , snd ( fst4 r ) , snd ( fst3 r ) , snd ( fst2 r ) , snd ( fst1 r ) , snd r ) 
- | dealer_ι_notify_addr_ v' => ( fst6 , v' , snd ( fst4 r ) , snd ( fst3 r ) , snd ( fst2 r ) , snd ( fst1 r ) , snd r ) 
- | dealer_ι_price_ v' => ( fst6 , snd ( fst5 r ) , v' , snd ( fst3 r ) , snd ( fst2 r ) , snd ( fst1 r ) , snd r ) 
- | dealer_ι_deals_limit_ v' => ( fst6 , snd ( fst5 r ) , snd ( fst4 r ) , v' , snd ( fst2 r ) , snd ( fst1 r ) , snd r ) 
- | dealer_ι_tons_cfg_ v' => ( fst6 , snd ( fst5 r ) , snd ( fst4 r ) , snd ( fst3 r ) , v' , snd ( fst1 r ) , snd r ) 
- | dealer_ι_sells_amount_ v' => ( fst6 , snd ( fst5 r ) , snd ( fst4 r ) , snd ( fst3 r ) , snd ( fst2 r ) , v' , snd r ) 
- | dealer_ι_buys_amount_ v' => ( fst6 , snd ( fst5 r ) , snd ( fst4 r ) , snd ( fst3 r ) , snd ( fst2 r ) , snd ( fst1 r ) , v' ) 
- end . 
-
- 
-Global Instance dealer_set_Record : PruvendoRecord dealerP dealerFields :=
-{
-  field_type := dealer_field_type; 
-  getPruvendoRecord := @dealer_get ;
-  setPruvendoRecord := @dealer_set ;
-}. 
 
  
 Class PruvendoRecord R F :=
@@ -1039,15 +664,572 @@ Class PruvendoRecord R F :=
   getPruvendoRecord: forall (f: F), R -> field_type f;
   setPruvendoRecord: forall (f: F), field_type f -> R -> R;
 }. 
-(* LocalState *) 
+Definition Tip3Config_set : forall (f: Tip3Config)  
+( v : match f with 
+| Tip3Config_ι_name => S 
+| Tip3Config_ι_symbol => S 
+| Tip3Config_ι_decimals => I8 
+| Tip3Config_ι_root_public_key => I256 
+| Tip3Config_ι_root_address => A 
+| Tip3Config_ι_code => C 
+
+end) (r:  Tip3ConfigP ) , Tip3ConfigP. 
+ intros. 
+ destruct r as  ((((( d1 , d2 ), d3), d4), d5), d6) . 
+ destruct f. 
+refine (v, d2, d3, d4, d5, d6) .
+ refine (d1, v, d3, d4, d5, d6) .
+ refine (d1, d2, v, d4, d5, d6) .
+ refine (d1, d2, d3, v, d5, d6) .
+ refine (d1, d2, d3, d4, v, d6) .
+ refine (d1, d2, d3, d4, d5, v) .
+ Defined.
+
+Instance Tip3Config_set_Record : PruvendoRecord Tip3ConfigP Tip3Config :=
+{
+  field_type := fun f => match f with 
+| Tip3Config_ι_name => S 
+| Tip3Config_ι_symbol => S 
+| Tip3Config_ι_decimals => I8 
+| Tip3Config_ι_root_public_key => I256 
+| Tip3Config_ι_root_address => A 
+| Tip3Config_ι_code => C 
+
+end;
+  getPruvendoRecord := @Tip3Config_get ;
+  setPruvendoRecord := @Tip3Config_set ;
+}. 
+Definition OrderRet_set : forall (f: OrderRet)  
+( v : match f with 
+| OrderRet_ι_err_code => I32 
+| OrderRet_ι_processed => I128 
+| OrderRet_ι_enqueued => I128 
+
+end) (r:  OrderRetP ) , OrderRetP. 
+ intros. 
+ destruct r as  (( d1 , d2 ), d3) . 
+ destruct f. 
+refine (v, d2, d3) .
+ refine (d1, v, d3) .
+ refine (d1, d2, v) .
+ Defined. 
+
+Instance OrderRet_set_Record : PruvendoRecord OrderRetP OrderRet :=
+{
+  field_type := fun f => match f with 
+| OrderRet_ι_err_code => I32 
+| OrderRet_ι_processed => I128 
+| OrderRet_ι_enqueued => I128 
+
+end;
+  getPruvendoRecord := @OrderRet_get ;
+  setPruvendoRecord := @OrderRet_set ;
+}. 
+Definition SellArgs_set : forall (f: SellArgs)  
+( v : match f with 
+| SellArgs_ι_amount => I128 
+| SellArgs_ι_receive_wallet => addr_std_fixedP 
+
+end) (r:  SellArgsP ) , SellArgsP. 
+ intros. 
+ destruct r as  ( d1 , d2 ) . 
+ destruct f. 
+refine (v, d2) .
+ refine (d1, v) .
+ Defined. 
+Instance SellArgs_set_Record : PruvendoRecord SellArgsP SellArgs :=
+{
+  field_type := fun f => match f with 
+| SellArgs_ι_amount => I128 
+| SellArgs_ι_receive_wallet => addr_std_fixedP 
+
+end;
+  getPruvendoRecord := @SellArgs_get ;
+  setPruvendoRecord := @SellArgs_set ;
+}. 
+Definition SellInfo_set : forall (f: SellInfo)  
+( v : match f with 
+| SellInfo_ι_original_amount => I128 
+| SellInfo_ι_amount => I128 
+| SellInfo_ι_account => I128 
+| SellInfo_ι_tip3_wallet => addr_std_fixedP 
+| SellInfo_ι_receive_wallet => addr_std_fixedP 
+| SellInfo_ι_lend_finish_time => I32 
+
+end) (r:  SellInfoP ) , SellInfoP. 
+ intros. 
+ destruct r as  ((((( d1 , d2 ), d3), d4), d5), d6) . 
+ destruct f. 
+refine (v, d2, d3, d4, d5, d6) .
+ refine (d1, v, d3, d4, d5, d6) .
+ refine (d1, d2, v, d4, d5, d6) .
+ refine (d1, d2, d3, v, d5, d6) .
+ refine (d1, d2, d3, d4, v, d6) .
+ refine (d1, d2, d3, d4, d5, v) .
+ Defined. 
+Instance SellInfo_set_Record : PruvendoRecord SellInfoP SellInfo :=
+{
+  field_type := fun f => match f with 
+| SellInfo_ι_original_amount => I128 
+| SellInfo_ι_amount => I128 
+| SellInfo_ι_account => I128 
+| SellInfo_ι_tip3_wallet => addr_std_fixedP 
+| SellInfo_ι_receive_wallet => addr_std_fixedP 
+| SellInfo_ι_lend_finish_time => I32 
+
+end;
+  getPruvendoRecord := @SellInfo_get ;
+  setPruvendoRecord := @SellInfo_set ;
+}. 
+
+Definition BuyInfo_set : forall (f: BuyInfo)  
+( v : match f with 
+| BuyInfo_ι_original_amount => I128 
+| BuyInfo_ι_amount => I128 
+| BuyInfo_ι_account => I128 
+| BuyInfo_ι_receive_tip3_wallet => addr_std_fixedP 
+| BuyInfo_ι_answer_addr => addr_std_fixedP 
+
+end) (r:  BuyInfoP ) , BuyInfoP. 
+ intros. 
+ destruct r as  (((( d1 , d2 ), d3), d4), d5) . 
+ destruct f. 
+refine (v, d2, d3, d4, d5) .
+ refine (d1, v, d3, d4, d5) .
+ refine (d1, d2, v, d4, d5) .
+ refine (d1, d2, d3, v, d5) .
+ refine (d1, d2, d3, d4, v) .
+Defined. 
+
+Instance BuyInfo_set_Record : PruvendoRecord BuyInfoP BuyInfo :=
+{
+  field_type := fun f => match f with 
+| BuyInfo_ι_original_amount => I128 
+| BuyInfo_ι_amount => I128 
+| BuyInfo_ι_account => I128 
+| BuyInfo_ι_receive_tip3_wallet => addr_std_fixedP 
+| BuyInfo_ι_answer_addr => addr_std_fixedP 
+
+end;
+  getPruvendoRecord := @BuyInfo_get ;
+  setPruvendoRecord := @BuyInfo_set ;
+}. 
+
+Definition DetailsInfo_set : forall (f: DetailsInfo)  
+( v : match f with 
+| DetailsInfo_ι_price => I128 
+| DetailsInfo_ι_min_amount => I128 
+| DetailsInfo_ι_sell_amount => I128 
+| DetailsInfo_ι_buy_amount => I128 
+
+end) (r:  DetailsInfoP ) , DetailsInfoP. 
+ intros. 
+ destruct r as  ((( d1 , d2 ), d3), d4) . 
+ destruct f. 
+refine (v, d2, d3, d4) .
+ refine (d1, v, d3, d4) .
+ refine (d1, d2, v, d4) .
+ refine (d1, d2, d3, v) .
+ Defined. 
+Instance DetailsInfo_set_Record : PruvendoRecord DetailsInfoP DetailsInfo :=
+{
+  field_type := fun f => match f with 
+| DetailsInfo_ι_price => I128 
+| DetailsInfo_ι_min_amount => I128 
+| DetailsInfo_ι_sell_amount => I128 
+| DetailsInfo_ι_buy_amount => I128 
+
+end;
+  getPruvendoRecord := @DetailsInfo_get ;
+  setPruvendoRecord := @DetailsInfo_set ;
+}. 
+
+Definition DPrice_set : forall (f: DPrice)  
+( v : match f with 
+| DPrice_ι_price_ => I128 
+| DPrice_ι_sells_amount_ => I128 
+| DPrice_ι_buys_amount_ => I128 
+| DPrice_ι_stock_ => addr_std_fixedP 
+| DPrice_ι_min_amount_ => I128 
+| DPrice_ι_deals_limit_ => I8 
+| DPrice_ι_notify_addr_ => IStockNotifyPtrP 
+| DPrice_ι_workchain_id_ => I8 
+| DPrice_ι_tons_cfg_ => TonsConfigP 
+| DPrice_ι_tip3cfg_ => Tip3ConfigP 
+
+end) (r:  DPriceP ) , DPriceP. 
+ intros. 
+ destruct r as  ((((((((( d1 , d2 ), d3), d4), d5), d6), d7), d8), d9), d10) . 
+ destruct f. 
+refine (v, d2, d3, d4, d5, d6, d7, d8, d9, d10) .
+ refine (d1, v, d3, d4, d5, d6, d7, d8, d9, d10) .
+ refine (d1, d2, v, d4, d5, d6, d7, d8, d9, d10) .
+ refine (d1, d2, d3, v, d5, d6, d7, d8, d9, d10) .
+ refine (d1, d2, d3, d4, v, d6, d7, d8, d9, d10) .
+ refine (d1, d2, d3, d4, d5, v, d7, d8, d9, d10) .
+ refine (d1, d2, d3, d4, d5, d6, v, d8, d9, d10) .
+ refine (d1, d2, d3, d4, d5, d6, d7, v, d9, d10) .
+ refine (d1, d2, d3, d4, d5, d6, d7, d8, v, d10) .
+ refine (d1, d2, d3, d4, d5, d6, d7, d8, d9, v) .
+ Defined. 
+
+Instance DPrice_set_Record : PruvendoRecord DPriceP DPrice :=
+{
+  field_type := fun f => match f with 
+| DPrice_ι_price_ => I128 
+| DPrice_ι_sells_amount_ => I128 
+| DPrice_ι_buys_amount_ => I128 
+| DPrice_ι_stock_ => addr_std_fixedP 
+| DPrice_ι_min_amount_ => I128 
+| DPrice_ι_deals_limit_ => I8 
+| DPrice_ι_notify_addr_ => IStockNotifyPtrP 
+| DPrice_ι_workchain_id_ => I8 
+| DPrice_ι_tons_cfg_ => TonsConfigP 
+| DPrice_ι_tip3cfg_ => Tip3ConfigP 
+
+end;
+  getPruvendoRecord := @DPrice_get ;
+  setPruvendoRecord := @DPrice_set ;
+}. 
+
+Definition TonsConfig_set : forall (f: TonsConfig)  
+( v : match f with 
+| TonsConfig_ι_transfer_tip3 => I128 
+| TonsConfig_ι_return_ownership => I128 
+| TonsConfig_ι_trading_pair_deploy => I128 
+| TonsConfig_ι_order_answer => I128 
+| TonsConfig_ι_process_queue => I128 
+| TonsConfig_ι_send_notify => I128 
+
+end) (r:  TonsConfigP ) , TonsConfigP. 
+ intros. 
+ destruct r as  ((((( d1 , d2 ), d3), d4), d5), d6) . 
+ destruct f. 
+refine (v, d2, d3, d4, d5, d6) .
+ refine (d1, v, d3, d4, d5, d6) .
+ refine (d1, d2, v, d4, d5, d6) .
+ refine (d1, d2, d3, v, d5, d6) .
+ refine (d1, d2, d3, d4, v, d6) .
+ refine (d1, d2, d3, d4, d5, v) .
+Defined. 
+
+Instance TonsConfig_set_Record : PruvendoRecord TonsConfigP TonsConfig :=
+{
+  field_type := fun f => match f with 
+| TonsConfig_ι_transfer_tip3 => I128 
+| TonsConfig_ι_return_ownership => I128 
+| TonsConfig_ι_trading_pair_deploy => I128 
+| TonsConfig_ι_order_answer => I128 
+| TonsConfig_ι_process_queue => I128 
+| TonsConfig_ι_send_notify => I128 
+
+end;
+  getPruvendoRecord := @TonsConfig_get ;
+  setPruvendoRecord := @TonsConfig_set ;
+}. 
+
+Definition DStock_set : forall (f: DStock)  
+( v : match f with 
+| DStock_ι_deployer_pubkey_ => I256 
+| DStock_ι_tons_cfg_ => TonsConfigP 
+| DStock_ι_min_amount_ => I128 
+| DStock_ι_deals_limit_ => I8 
+| DStock_ι_notify_addr_ => A 
+
+end) (r:  DStockP ) , DStockP. 
+ intros. 
+ destruct r as  (((( d1 , d2 ), d3), d4), d5) . 
+ destruct f. 
+refine (v, d2, d3, d4, d5) .
+ refine (d1, v, d3, d4, d5) .
+ refine (d1, d2, v, d4, d5) .
+ refine (d1, d2, d3, v, d5) .
+ refine (d1, d2, d3, d4, v) .
+Defined. 
+
+Instance DStock_set_Record : PruvendoRecord DStockP DStock :=
+{
+  field_type := fun f => match f with 
+| DStock_ι_deployer_pubkey_ => I256 
+| DStock_ι_tons_cfg_ => TonsConfigP 
+| DStock_ι_min_amount_ => I128 
+| DStock_ι_deals_limit_ => I8 
+| DStock_ι_notify_addr_ => A 
+
+end;
+  getPruvendoRecord := @DStock_get ;
+  setPruvendoRecord := @DStock_set ;
+}. 
+
+Definition DTradingPair_set : forall (f: DTradingPair)  
+( v : match f with 
+| DTradingPair_ι_stock_addr_ => A 
+| DTradingPair_ι_tip3_root_ => A 
+| DTradingPair_ι_deploy_value_ => I128 
+
+end) (r:  DTradingPairP ) , DTradingPairP. 
+ intros. 
+ destruct r as  (( d1 , d2 ), d3) . 
+ destruct f. 
+refine (v, d2, d3) .
+ refine (d1, v, d3) .
+ refine (d1, d2, v) .
+Defined. 
+
+Instance DTradingPair_set_Record : PruvendoRecord DTradingPairP DTradingPair :=
+{
+  field_type := fun f => match f with 
+| DTradingPair_ι_stock_addr_ => A 
+| DTradingPair_ι_tip3_root_ => A 
+| DTradingPair_ι_deploy_value_ => I128 
+
+end;
+  getPruvendoRecord := @DTradingPair_get ;
+  setPruvendoRecord := @DTradingPair_set ;
+}. 
+
+Definition FLeXSellArgsAddrs_set : forall (f: FLeXSellArgsAddrs)  
+( v : match f with 
+| FLeXSellArgsAddrs_ι_my_tip3_addr => A 
+| FLeXSellArgsAddrs_ι_receive_wallet => A 
+
+end) (r:  FLeXSellArgsAddrsP ) , FLeXSellArgsAddrsP. 
+ intros. 
+ destruct r as  ( d1 , d2 ) . 
+ destruct f. 
+refine (v, d2) .
+ refine (d1, v) .
+Defined. 
+
+Instance FLeXSellArgsAddrs_set_Record : PruvendoRecord FLeXSellArgsAddrsP FLeXSellArgsAddrs :=
+{
+  field_type := fun f => match f with 
+| FLeXSellArgsAddrs_ι_my_tip3_addr => A 
+| FLeXSellArgsAddrs_ι_receive_wallet => A 
+
+end;
+  getPruvendoRecord := @FLeXSellArgsAddrs_get ;
+  setPruvendoRecord := @FLeXSellArgsAddrs_set ;
+}. 
+
+Definition FLeXSellArgs_set : forall (f: FLeXSellArgs)  
+( v : match f with 
+| FLeXSellArgs_ι_price => I128 
+| FLeXSellArgs_ι_amount => I128 
+| FLeXSellArgs_ι_lend_finish_time => I32 
+| FLeXSellArgs_ι_min_amount => I128 
+| FLeXSellArgs_ι_deals_limit => I8 
+| FLeXSellArgs_ι_tons_value => I128 
+| FLeXSellArgs_ι_price_code => C 
+
+end) (r:  FLeXSellArgsP ) , FLeXSellArgsP. 
+ intros. 
+ destruct r as  (((((( d1 , d2 ), d3), d4), d5), d6), d7) . 
+ destruct f. 
+refine (v, d2, d3, d4, d5, d6, d7) .
+ refine (d1, v, d3, d4, d5, d6, d7) .
+ refine (d1, d2, v, d4, d5, d6, d7) .
+ refine (d1, d2, d3, v, d5, d6, d7) .
+ refine (d1, d2, d3, d4, v, d6, d7) .
+ refine (d1, d2, d3, d4, d5, v, d7) .
+ refine (d1, d2, d3, d4, d5, d6, v) .
+Defined. 
+
+Instance FLeXSellArgs_set_Record : PruvendoRecord FLeXSellArgsP FLeXSellArgs :=
+{
+  field_type := fun f => match f with 
+| FLeXSellArgs_ι_price => I128 
+| FLeXSellArgs_ι_amount => I128 
+| FLeXSellArgs_ι_lend_finish_time => I32 
+| FLeXSellArgs_ι_min_amount => I128 
+| FLeXSellArgs_ι_deals_limit => I8 
+| FLeXSellArgs_ι_tons_value => I128 
+| FLeXSellArgs_ι_price_code => C 
+
+end;
+  getPruvendoRecord := @FLeXSellArgs_get ;
+  setPruvendoRecord := @FLeXSellArgs_set ;
+}. 
+
+Definition FLeXBuyArgs_set : forall (f: FLeXBuyArgs)  
+( v : match f with 
+| FLeXBuyArgs_ι_price => I128 
+| FLeXBuyArgs_ι_amount => I128 
+| FLeXBuyArgs_ι_min_amount => I128 
+| FLeXBuyArgs_ι_deals_limit => I8 
+| FLeXBuyArgs_ι_deploy_value => I128 
+| FLeXBuyArgs_ι_price_code => C 
+| FLeXBuyArgs_ι_my_tip3_addr => A 
+
+end) (r:  FLeXBuyArgsP ) , FLeXBuyArgsP. 
+ intros. 
+ destruct r as  (((((( d1 , d2 ), d3), d4), d5), d6), d7) . 
+ destruct f. 
+refine (v, d2, d3, d4, d5, d6, d7) .
+ refine (d1, v, d3, d4, d5, d6, d7) .
+ refine (d1, d2, v, d4, d5, d6, d7) .
+ refine (d1, d2, d3, v, d5, d6, d7) .
+ refine (d1, d2, d3, d4, v, d6, d7) .
+ refine (d1, d2, d3, d4, d5, v, d7) .
+ refine (d1, d2, d3, d4, d5, d6, v) .
+Defined. 
+
+Instance FLeXBuyArgs_set_Record : PruvendoRecord FLeXBuyArgsP FLeXBuyArgs :=
+{
+  field_type := fun f => match f with 
+| FLeXBuyArgs_ι_price => I128 
+| FLeXBuyArgs_ι_amount => I128 
+| FLeXBuyArgs_ι_min_amount => I128 
+| FLeXBuyArgs_ι_deals_limit => I8 
+| FLeXBuyArgs_ι_deploy_value => I128 
+| FLeXBuyArgs_ι_price_code => C 
+| FLeXBuyArgs_ι_my_tip3_addr => A 
+
+end;
+  getPruvendoRecord := @FLeXBuyArgs_get ;
+  setPruvendoRecord := @FLeXBuyArgs_set ;
+}. 
+
+Definition FLeXCancelArgs_set : forall (f: FLeXCancelArgs)  
+( v : match f with 
+| FLeXCancelArgs_ι_price => I128 
+| FLeXCancelArgs_ι_min_amount => I128 
+| FLeXCancelArgs_ι_deals_limit => I8 
+| FLeXCancelArgs_ι_value => I128 
+| FLeXCancelArgs_ι_price_code => C 
+
+end) (r:  FLeXCancelArgsP ) , FLeXCancelArgsP. 
+ intros. 
+ destruct r as  (((( d1 , d2 ), d3), d4), d5) . 
+ destruct f. 
+refine (v, d2, d3, d4, d5) .
+ refine (d1, v, d3, d4, d5) .
+ refine (d1, d2, v, d4, d5) .
+ refine (d1, d2, d3, v, d5) .
+ refine (d1, d2, d3, d4, v) .
+Defined. 
+
+Instance FLeXCancelArgs_set_Record : PruvendoRecord FLeXCancelArgsP FLeXCancelArgs :=
+{
+  field_type := fun f => match f with 
+| FLeXCancelArgs_ι_price => I128 
+| FLeXCancelArgs_ι_min_amount => I128 
+| FLeXCancelArgs_ι_deals_limit => I8 
+| FLeXCancelArgs_ι_value => I128 
+| FLeXCancelArgs_ι_price_code => C 
+
+end;
+  getPruvendoRecord := @FLeXCancelArgs_get ;
+  setPruvendoRecord := @FLeXCancelArgs_set ;
+}. 
+
+Definition DFLeXClient_set : forall (f: DFLeXClient)  
+( v : match f with 
+| DFLeXClient_ι_owner_ => I256 
+| DFLeXClient_ι_trading_pair_code_ => C 
+| DFLeXClient_ι_workchain_id_ => I8 
+| DFLeXClient_ι_tons_cfg_ => TonsConfigP 
+| DFLeXClient_ι_stock_ => A 
+| DFLeXClient_ι_notify_addr_ => A 
+
+end) (r:  DFLeXClientP ) , DFLeXClientP. 
+ intros. 
+ destruct r as  ((((( d1 , d2 ), d3), d4), d5), d6) . 
+ destruct f. 
+refine (v, d2, d3, d4, d5, d6) .
+ refine (d1, v, d3, d4, d5, d6) .
+ refine (d1, d2, v, d4, d5, d6) .
+ refine (d1, d2, d3, v, d5, d6) .
+ refine (d1, d2, d3, d4, v, d6) .
+ refine (d1, d2, d3, d4, d5, v) .
+Defined. 
+
+Instance DFLeXClient_set_Record : PruvendoRecord DFLeXClientP DFLeXClient :=
+{
+  field_type := fun f => match f with 
+| DFLeXClient_ι_owner_ => I256 
+| DFLeXClient_ι_trading_pair_code_ => C 
+| DFLeXClient_ι_workchain_id_ => I8 
+| DFLeXClient_ι_tons_cfg_ => TonsConfigP 
+| DFLeXClient_ι_stock_ => A 
+| DFLeXClient_ι_notify_addr_ => A 
+
+end;
+  getPruvendoRecord := @DFLeXClient_get ;
+  setPruvendoRecord := @DFLeXClient_set ;
+}. 
+
+Definition process_ret_set : forall (f: process_ret)  
+( v : match f with 
+| process_ret_ι_sells_amount => I128 
+| process_ret_ι_buys_amount => I128 
+
+end) (r:  process_retP ) , process_retP. 
+ intros. 
+ destruct r as  ( d1 , d2 ) . 
+ destruct f. 
+refine (v, d2) .
+ refine (d1, v) .
+Defined. 
+
+Instance process_ret_set_Record : PruvendoRecord process_retP process_ret :=
+{
+  field_type := fun f => match f with 
+| process_ret_ι_sells_amount => I128 
+| process_ret_ι_buys_amount => I128 
+
+end;
+  getPruvendoRecord := @process_ret_get ;
+  setPruvendoRecord := @process_ret_set ;
+}. 
+
+Definition dealer_set : forall (f: dealer)  
+( v : match f with 
+| dealer_ι_tip3root_ => A 
+| dealer_ι_notify_addr_ => IStockNotifyPtrP 
+| dealer_ι_price_ => I128 
+| dealer_ι_deals_limit_ => I 
+| dealer_ι_tons_cfg_ => TonsConfigP 
+| dealer_ι_sells_amount_ => I128 
+| dealer_ι_buys_amount_ => I128 
+
+end) (r:  dealerP ) , dealerP. 
+ intros. 
+ destruct r as  (((((( d1 , d2 ), d3), d4), d5), d6), d7) . 
+ destruct f. 
+refine (v, d2, d3, d4, d5, d6, d7) .
+ refine (d1, v, d3, d4, d5, d6, d7) .
+ refine (d1, d2, v, d4, d5, d6, d7) .
+ refine (d1, d2, d3, v, d5, d6, d7) .
+ refine (d1, d2, d3, d4, v, d6, d7) .
+ refine (d1, d2, d3, d4, d5, v, d7) .
+ refine (d1, d2, d3, d4, d5, d6, v) .
+Defined. 
+
+Instance dealer_set_Record : PruvendoRecord dealerP dealer :=
+{
+  field_type := fun f => match f with 
+| dealer_ι_tip3root_ => A 
+| dealer_ι_notify_addr_ => IStockNotifyPtrP 
+| dealer_ι_price_ => I128 
+| dealer_ι_deals_limit_ => I 
+| dealer_ι_tons_cfg_ => TonsConfigP 
+| dealer_ι_sells_amount_ => I128 
+| dealer_ι_buys_amount_ => I128 
+
+end;
+  getPruvendoRecord := @dealer_get ;
+  setPruvendoRecord := @dealer_set ;
+}. 
+
+
 Notation "'{$$' r 'With' y ':=' v '$$}'" := (@setPruvendoRecord _ _ _ y v r) : struct_scope.
  
 Lemma no_Tip3Config_eq : forall (f1 f2: Tip3Config) (v2: field_type f2) (r : Tip3ConfigP ) ,  
 f1 <> f2 -> 
 f1 {$$ r With f2 := v2 $$} = f1 r.
 Proof.
-intros.
-destruct r. destruct p.
+intros. destruct r as  ((((( d1 , d2 ), d3), d4), d5), d6) .
 destruct f1; destruct f2; auto; try contradiction.
 Qed.
 
@@ -1055,15 +1237,16 @@ Lemma Tip3Config_eq : forall (f2: Tip3Config) (v2: field_type f2) (r : Tip3Confi
 f2 {$$ r With f2 := v2 $$} = v2.
 Proof.
 intros.
-destruct r. destruct p.
+destruct r as  ((((( d1 , d2 ), d3), d4), d5), d6) .
 destruct f2; auto.
-Qed. 
+Qed.
+
 Lemma no_OrderRet_eq : forall (f1 f2: OrderRet) (v2: field_type f2) (r : OrderRetP ) ,  
 f1 <> f2 -> 
 f1 {$$ r With f2 := v2 $$} = f1 r.
 Proof.
 intros.
-destruct r. destruct p.
+destruct r as  (( d1 , d2 ), d3) .
 destruct f1; destruct f2; auto; try contradiction.
 Qed.
 
@@ -1071,15 +1254,16 @@ Lemma OrderRet_eq : forall (f2: OrderRet) (v2: field_type f2) (r : OrderRetP ) ,
 f2 {$$ r With f2 := v2 $$} = v2.
 Proof.
 intros.
-destruct r. destruct p.
+destruct r as  (( d1 , d2 ), d3) .
 destruct f2; auto.
-Qed. 
+Qed.
+ 
 Lemma no_SellArgs_eq : forall (f1 f2: SellArgs) (v2: field_type f2) (r : SellArgsP ) ,  
 f1 <> f2 -> 
 f1 {$$ r With f2 := v2 $$} = f1 r.
 Proof.
 intros.
-destruct r. destruct p.
+destruct r as  ( d1 , d2 ) .
 destruct f1; destruct f2; auto; try contradiction.
 Qed.
 
@@ -1087,15 +1271,15 @@ Lemma SellArgs_eq : forall (f2: SellArgs) (v2: field_type f2) (r : SellArgsP ) ,
 f2 {$$ r With f2 := v2 $$} = v2.
 Proof.
 intros.
-destruct r. destruct p.
+destruct r as  ( d1 , d2 ) .
 destruct f2; auto.
-Qed. 
+Qed.
+ 
 Lemma no_SellInfo_eq : forall (f1 f2: SellInfo) (v2: field_type f2) (r : SellInfoP ) ,  
 f1 <> f2 -> 
 f1 {$$ r With f2 := v2 $$} = f1 r.
 Proof.
-intros.
-destruct r. destruct p.
+intros. destruct r as  ((((( d1 , d2 ), d3), d4), d5), d6) .
 destruct f1; destruct f2; auto; try contradiction.
 Qed.
 
@@ -1103,15 +1287,16 @@ Lemma SellInfo_eq : forall (f2: SellInfo) (v2: field_type f2) (r : SellInfoP ) ,
 f2 {$$ r With f2 := v2 $$} = v2.
 Proof.
 intros.
-destruct r. destruct p.
+destruct r as  ((((( d1 , d2 ), d3), d4), d5), d6) .
 destruct f2; auto.
 Qed. 
+
 Lemma no_BuyInfo_eq : forall (f1 f2: BuyInfo) (v2: field_type f2) (r : BuyInfoP ) ,  
 f1 <> f2 -> 
 f1 {$$ r With f2 := v2 $$} = f1 r.
 Proof.
 intros.
-destruct r. destruct p.
+destruct r as  (((( d1 , d2 ), d3), d4), d5).
 destruct f1; destruct f2; auto; try contradiction.
 Qed.
 
@@ -1119,15 +1304,16 @@ Lemma BuyInfo_eq : forall (f2: BuyInfo) (v2: field_type f2) (r : BuyInfoP ) ,
 f2 {$$ r With f2 := v2 $$} = v2.
 Proof.
 intros.
-destruct r. destruct p.
+destruct r as  (((( d1 , d2 ), d3), d4), d5).
 destruct f2; auto.
 Qed. 
+
 Lemma no_DetailsInfo_eq : forall (f1 f2: DetailsInfo) (v2: field_type f2) (r : DetailsInfoP ) ,  
 f1 <> f2 -> 
 f1 {$$ r With f2 := v2 $$} = f1 r.
 Proof.
 intros.
-destruct r. destruct p.
+destruct r as  ((( d1 , d2 ), d3), d4).
 destruct f1; destruct f2; auto; try contradiction.
 Qed.
 
@@ -1135,15 +1321,17 @@ Lemma DetailsInfo_eq : forall (f2: DetailsInfo) (v2: field_type f2) (r : Details
 f2 {$$ r With f2 := v2 $$} = v2.
 Proof.
 intros.
-destruct r. destruct p.
+destruct r as  ((( d1 , d2 ), d3), d4).
 destruct f2; auto.
 Qed. 
+
 Lemma no_DPrice_eq : forall (f1 f2: DPrice) (v2: field_type f2) (r : DPriceP ) ,  
 f1 <> f2 -> 
 f1 {$$ r With f2 := v2 $$} = f1 r.
 Proof.
 intros.
-destruct r. destruct p.
+ destruct r as  ((((((((( d1 , d2 ), d3), d4), d5), d6), d7), d8), d9), d10) . 
+
 destruct f1; destruct f2; auto; try contradiction.
 Qed.
 
@@ -1151,15 +1339,16 @@ Lemma DPrice_eq : forall (f2: DPrice) (v2: field_type f2) (r : DPriceP ) ,
 f2 {$$ r With f2 := v2 $$} = v2.
 Proof.
 intros.
-destruct r. destruct p.
+ destruct r as  ((((((((( d1 , d2 ), d3), d4), d5), d6), d7), d8), d9), d10) . 
 destruct f2; auto.
 Qed. 
+
 Lemma no_TonsConfig_eq : forall (f1 f2: TonsConfig) (v2: field_type f2) (r : TonsConfigP ) ,  
 f1 <> f2 -> 
 f1 {$$ r With f2 := v2 $$} = f1 r.
 Proof.
 intros.
-destruct r. destruct p.
+destruct r as  ((((( d1 , d2 ), d3), d4), d5), d6).
 destruct f1; destruct f2; auto; try contradiction.
 Qed.
 
@@ -1167,15 +1356,16 @@ Lemma TonsConfig_eq : forall (f2: TonsConfig) (v2: field_type f2) (r : TonsConfi
 f2 {$$ r With f2 := v2 $$} = v2.
 Proof.
 intros.
-destruct r. destruct p.
+destruct r as  ((((( d1 , d2 ), d3), d4), d5), d6).
 destruct f2; auto.
 Qed. 
+
 Lemma no_DStock_eq : forall (f1 f2: DStock) (v2: field_type f2) (r : DStockP ) ,  
 f1 <> f2 -> 
 f1 {$$ r With f2 := v2 $$} = f1 r.
 Proof.
 intros.
-destruct r. destruct p.
+destruct r as  (((( d1 , d2 ), d3), d4), d5).
 destruct f1; destruct f2; auto; try contradiction.
 Qed.
 
@@ -1183,15 +1373,16 @@ Lemma DStock_eq : forall (f2: DStock) (v2: field_type f2) (r : DStockP ) ,
 f2 {$$ r With f2 := v2 $$} = v2.
 Proof.
 intros.
-destruct r. destruct p.
+destruct r as  (((( d1 , d2 ), d3), d4), d5).
 destruct f2; auto.
 Qed. 
+
 Lemma no_DTradingPair_eq : forall (f1 f2: DTradingPair) (v2: field_type f2) (r : DTradingPairP ) ,  
 f1 <> f2 -> 
 f1 {$$ r With f2 := v2 $$} = f1 r.
 Proof.
 intros.
-destruct r. destruct p.
+destruct r as  (( d1 , d2 ), d3).
 destruct f1; destruct f2; auto; try contradiction.
 Qed.
 
@@ -1199,15 +1390,16 @@ Lemma DTradingPair_eq : forall (f2: DTradingPair) (v2: field_type f2) (r : DTrad
 f2 {$$ r With f2 := v2 $$} = v2.
 Proof.
 intros.
-destruct r. destruct p.
+destruct r as  (( d1 , d2 ), d3).
 destruct f2; auto.
 Qed. 
+
 Lemma no_FLeXSellArgsAddrs_eq : forall (f1 f2: FLeXSellArgsAddrs) (v2: field_type f2) (r : FLeXSellArgsAddrsP ) ,  
 f1 <> f2 -> 
 f1 {$$ r With f2 := v2 $$} = f1 r.
 Proof.
 intros.
-destruct r. destruct p.
+destruct r as  ( d1 , d2 ).
 destruct f1; destruct f2; auto; try contradiction.
 Qed.
 
@@ -1215,15 +1407,16 @@ Lemma FLeXSellArgsAddrs_eq : forall (f2: FLeXSellArgsAddrs) (v2: field_type f2) 
 f2 {$$ r With f2 := v2 $$} = v2.
 Proof.
 intros.
-destruct r. destruct p.
+destruct r as  ( d1 , d2 ).
 destruct f2; auto.
 Qed. 
+
 Lemma no_FLeXSellArgs_eq : forall (f1 f2: FLeXSellArgs) (v2: field_type f2) (r : FLeXSellArgsP ) ,  
 f1 <> f2 -> 
 f1 {$$ r With f2 := v2 $$} = f1 r.
 Proof.
 intros.
-destruct r. destruct p.
+destruct r as  (((((( d1 , d2 ), d3), d4), d5), d6), d7).
 destruct f1; destruct f2; auto; try contradiction.
 Qed.
 
@@ -1231,15 +1424,16 @@ Lemma FLeXSellArgs_eq : forall (f2: FLeXSellArgs) (v2: field_type f2) (r : FLeXS
 f2 {$$ r With f2 := v2 $$} = v2.
 Proof.
 intros.
-destruct r. destruct p.
+destruct r as  (((((( d1 , d2 ), d3), d4), d5), d6), d7).
 destruct f2; auto.
 Qed. 
+
 Lemma no_FLeXBuyArgs_eq : forall (f1 f2: FLeXBuyArgs) (v2: field_type f2) (r : FLeXBuyArgsP ) ,  
 f1 <> f2 -> 
 f1 {$$ r With f2 := v2 $$} = f1 r.
 Proof.
 intros.
-destruct r. destruct p.
+destruct r as  (((((( d1 , d2 ), d3), d4), d5), d6), d7).
 destruct f1; destruct f2; auto; try contradiction.
 Qed.
 
@@ -1247,15 +1441,16 @@ Lemma FLeXBuyArgs_eq : forall (f2: FLeXBuyArgs) (v2: field_type f2) (r : FLeXBuy
 f2 {$$ r With f2 := v2 $$} = v2.
 Proof.
 intros.
-destruct r. destruct p.
+destruct r as  (((((( d1 , d2 ), d3), d4), d5), d6), d7).
 destruct f2; auto.
 Qed. 
+
 Lemma no_FLeXCancelArgs_eq : forall (f1 f2: FLeXCancelArgs) (v2: field_type f2) (r : FLeXCancelArgsP ) ,  
 f1 <> f2 -> 
 f1 {$$ r With f2 := v2 $$} = f1 r.
 Proof.
 intros.
-destruct r. destruct p.
+destruct r as  (((( d1 , d2 ), d3), d4), d5).
 destruct f1; destruct f2; auto; try contradiction.
 Qed.
 
@@ -1263,15 +1458,16 @@ Lemma FLeXCancelArgs_eq : forall (f2: FLeXCancelArgs) (v2: field_type f2) (r : F
 f2 {$$ r With f2 := v2 $$} = v2.
 Proof.
 intros.
-destruct r. destruct p.
+destruct r as  (((( d1 , d2 ), d3), d4), d5).
 destruct f2; auto.
 Qed. 
+
 Lemma no_DFLeXClient_eq : forall (f1 f2: DFLeXClient) (v2: field_type f2) (r : DFLeXClientP ) ,  
 f1 <> f2 -> 
 f1 {$$ r With f2 := v2 $$} = f1 r.
 Proof.
 intros.
-destruct r. destruct p.
+destruct r as  ((((( d1 , d2 ), d3), d4), d5), d6).
 destruct f1; destruct f2; auto; try contradiction.
 Qed.
 
@@ -1279,7 +1475,7 @@ Lemma DFLeXClient_eq : forall (f2: DFLeXClient) (v2: field_type f2) (r : DFLeXCl
 f2 {$$ r With f2 := v2 $$} = v2.
 Proof.
 intros.
-destruct r. destruct p.
+destruct r as  ((((( d1 , d2 ), d3), d4), d5), d6).
 destruct f2; auto.
 Qed. 
 
@@ -1288,7 +1484,7 @@ f1 <> f2 ->
 f1 {$$ r With f2 := v2 $$} = f1 r.
 Proof.
 intros.
-destruct r. destruct p.
+destruct r as  ( d1 , d2 ).
 destruct f1; destruct f2; auto; try contradiction.
 Qed.
 
@@ -1296,18 +1492,16 @@ Lemma process_ret_eq : forall (f2: process_ret) (v2: field_type f2) (r : process
 f2 {$$ r With f2 := v2 $$} = v2.
 Proof.
 intros.
-destruct r. destruct p.
+destruct r as  ( d1 , d2 ).
 destruct f2; auto.
 Qed. 
-
-
 
 Lemma no_dealer_eq : forall (f1 f2: dealer) (v2: field_type f2) (r : dealerP ) ,  
 f1 <> f2 -> 
 f1 {$$ r With f2 := v2 $$} = f1 r.
 Proof.
 intros.
-destruct r. destruct p.
+destruct r as  (((((( d1 , d2 ), d3), d4), d5), d6), d7).
 destruct f1; destruct f2; auto; try contradiction.
 Qed.
 
@@ -1315,9 +1509,38 @@ Lemma dealer_eq : forall (f2: dealer) (v2: field_type f2) (r : dealerP ) ,
 f2 {$$ r With f2 := v2 $$} = v2.
 Proof.
 intros.
-destruct r. destruct p.
+destruct r as  (((((( d1 , d2 ), d3), d4), d5), d6), d7).
 destruct f2; auto.
 Qed. 
+
+
+Notation " 'fst0' x " := ( x ) (at level 60, right associativity).
+Notation " 'fst1' x " := ( fst ( fst0 x ) ) (at level 60, right associativity).
+Notation " 'fst2' x " := ( fst ( fst1 x ) ) (at level 60, right associativity).
+Notation " 'fst3' x " := ( fst ( fst2 x ) ) (at level 60, right associativity).
+Notation " 'fst4' x " := ( fst ( fst3 x ) ) (at level 60, right associativity).
+Notation " 'fst5' x " := ( fst ( fst4 x ) ) (at level 60, right associativity).
+Notation " 'fst6' x " := ( fst ( fst5 x ) ) (at level 60, right associativity).
+Notation " 'fst7' x " := ( fst ( fst6 x ) ) (at level 60, right associativity).
+Notation " 'fst8' x " := ( fst ( fst7 x ) ) (at level 60, right associativity).
+Notation " 'fst9' x " := ( fst ( fst8 x ) ) (at level 60, right associativity).
+Notation " 'fst10' x " := ( fst ( fst9 x ) ) (at level 60, right associativity).
+Notation " 'fst11' x " := ( fst ( fst10 x ) ) (at level 60, right associativity).
+Notation " 'fst12' x " := ( fst ( fst11 x ) ) (at level 60, right associativity).
+Notation " 'fst13' x " := ( fst ( fst12 x ) ) (at level 60, right associativity).
+Notation " 'fst14' x " := ( fst ( fst13 x ) ) (at level 60, right associativity).
+Notation " 'fst15' x " := ( fst ( fst14 x ) ) (at level 60, right associativity).
+Notation " 'fst16' x " := ( fst ( fst15 x ) ) (at level 60, right associativity).
+Notation " 'fst17' x " := ( fst ( fst16 x ) ) (at level 60, right associativity).
+Notation " 'fst18' x " := ( fst ( fst17 x ) ) (at level 60, right associativity).
+Notation " 'fst19' x " := ( fst ( fst18 x ) ) (at level 60, right associativity).
+Notation " 'fst20' x " := ( fst ( fst19 x ) ) (at level 60, right associativity).
+
+Compute fst6 ("1","2","3","4","5","6","7")%string.
+
+
+
+
 
 
 
